Corrected a bug in function and wrote the first spec

src/AByteFile.v
@@ -76,186 +76,186 @@ Definition get_block_size: valu -> nat.
 Proof. Admitted.
 
 
-Fixpoint read_from_block (l: list byte) (off len: nat) : list byte :=
+Fixpoint get_sublist {A:Type}(l: list A) (off len: nat) : list A :=
   match off with
   | O => match len with 
           | O => nil
           | S len' => match l with
                       | nil => nil
-                      | b::l' => b::(read_from_block l' O len')
+                      | b::l' => b::(get_sublist l' O len')
                       end
           end
   | S off'=> match l with
               | nil => nil
-              | b::l' => (read_from_block l' off' len)
+              | b::l' => (get_sublist l' off' len)
               end
   end.
+
   
 (*Ugly but at least compiling*)
 
 Definition read_bytes {T} lxp ixp inum (off len:nat) fms rx : prog T :=
-If (lt_dec 0 len) {                                           (* if read length > 0 *)
+If (lt_dec 0 len)                        (* if read length > 0 *)
+{                    
   let^ (fms, flen) <- BFILE.getlen lxp ixp inum fms;          (* get file length *)
-  If (lt_dec off flen) {                                      (* if offset is inside file *)
-    If(le_dec (off+len) flen) {                               (* if you can read the whole length *)
-      let^ (fms, first_block) <- BFILE.read lxp ixp inum off fms;   (* get first block *)
-      let block_size := (get_block_size first_block) in             (* get block size *)
-      let relative_off := (modulo off block_size) in          (* calculate block offset *)
-      If(le_dec (relative_off + len) block_size) {            (* if whole data is in this block *)
-        let data := (read_from_block                          (* read the data and return as list byte *)
-        (valu_to_list first_block) relative_off len) in
+  If (lt_dec off flen)                   (* if offset is inside file *)
+  {                    
+    If(le_dec (off+len) flen)     (* if you can read the whole length *)
+    {                           
+      let^ (fms, block0) <- BFILE.read lxp ixp inum 0 fms;        (* get block 0*)
+      let block_size := (get_block_size block0) in            (* get block size *)
+      let block_off := (off / block_size) in              (* calculate block offset *)
+      let byte_off := (modulo off block_size) in          (* calculate byte offset *)
+      let^ (fms, first_block) <- BFILE.read lxp ixp inum block_off fms;   (* get first block *)
+      If(le_dec (byte_off + len) block_size)             (* if whole data is in this block *)
+      {
+        let data := (get_sublist                          (* read the data and return as list byte *)
+        (valu_to_list first_block) byte_off len) in
         rx ^(fms, data)
-      } else {                                                (* If data is in more than one block *)
-        let data_init := (read_from_block                     (* read as much as you can from this block *)
-        (valu_to_list first_block) relative_off         
-         (block_size - relative_off)) in
-        let off_remain := (off + (block_size - relative_off)) in  (* offset of remaining part *)
-        let len_remain := (len - (block_size - relative_off)) in  (* length of remaining part *)
+      } 
+      else                                            (* If data is in more than one block *)
+      {     
+        let data_init := (get_sublist                     (* read as much as you can from this block *)
+        (valu_to_list first_block) byte_off         
+         (block_size - byte_off)) in
+        let block_off := (block_off +1) in                      (* offset of remaining part *)
+        let len_remain := (len - (block_size - byte_off)) in  (* length of remaining part *)
         let num_of_full_blocks := (len_remain / block_size) in (* number of full blocks in length *)
-        
-        (* for loop notation can't find implicit arguments*)
-        (*let^ (data) <- ForN i <  num_of_full_blocks
-        Ghost [ len_remain ]
-        Loopvar [data]
-        Continuation lrx
-        Invariant
-         (fun _ => True)
-        OnCrash
-         (fun _ => True)
-        Begin
-          let^ (fms, block) <- BFILE.read lxp ixp inum (off_remain + i*block_size) fms;
-          lrx ^(data++(read_from_block (valu_to_list block) 0 block_size))
-        Rof ^(data_init);*)
         
         (*for loop for reading those full blocks *)
         let^ (data) <- (ForN_ (fun i =>
           (pair_args_helper (fun data (_:unit) => (fun lrx => 
           
-          let^ (fms, block) <- BFILE.read lxp ixp inum (off_remain + i*block_size) fms; (* get i'th block *)
-          lrx ^(data++(read_from_block (valu_to_list block) 0 block_size))%list (* append its contents *)
+          let^ (fms, block) <- BFILE.read lxp ixp inum (block_off + i) fms; (* get i'th block *)
+          lrx ^(data++(get_sublist (valu_to_list block) 0 block_size))%list (* append its contents *)
           
           )))) 0 num_of_full_blocks
         (fun _:nat => (fun _ => (fun _ => (fun _ => (fun _ => True)%pred)))) (* trivial invariant *)
         (fun _:nat => (fun _ => (fun _ => True)%pred))) ^(nil);             (* trivial crashpred *)
         
-        let off_final := (off_remain + num_of_full_blocks * block_size) in (* offset of final block *)
+        let off_final := (block_off + num_of_full_blocks * block_size) in (* offset of final block *)
         let len_final := (len_remain - num_of_full_blocks * block_size) in (* final remaining length *)
-        let^ (fms, last_block) <- BFILE.read lxp ixp inum off_remain fms;   (* get final block *)
-        let data_final := (read_from_block (valu_to_list last_block) 0 len_final) in (* get final block data *)
+        let^ (fms, last_block) <- BFILE.read lxp ixp inum off_final fms;   (* get final block *)
+        let data_final := (get_sublist (valu_to_list last_block) 0 len_final) in (* get final block data *)
         rx ^(fms, data_init++data++data_final)%list                  (* append everything and return *)
-        }
-      } else {                                                  (* If you cannot read the whole length *)
-        let len:= (flen - off) in                               (* set length to remaining length of file *)
-        let^ (fms, first_block) <- BFILE.read lxp ixp inum off fms;   (* get first block *)
-        let block_size := (get_block_size first_block) in             (* get block size *)
-        let relative_off := (modulo off block_size) in          (* calculate block offset *)
-        If(le_dec (relative_off + len) block_size) {            (* if whole data is in this block *)
-          let data := (read_from_block                          (* read the data and return as list byte *)
-          (valu_to_list first_block) relative_off len) in
-          rx ^(fms, data)
-        } else {                                                (* If data is in more than one block *)
-            let data_init := (read_from_block                     (* read as much as you can from this block *)
-            (valu_to_list first_block) relative_off  
-             (block_size - relative_off)) in
-            let off_remain := (off + (block_size - relative_off)) in  (* offset of remaining part *)
-            let len_remain := (len - (block_size - relative_off)) in  (* length of remaining part *)
-            let num_of_full_blocks := (len_remain / block_size) in (* number of full blocks in length *)
-            
-            (* for loop notation can't find implicit arguments*)
-            (*let^ (data) <- ForN i <  num_of_full_blocks 
-            Ghost [ len_remain ]
-            Loopvar [data]
-            Continuation lrx
-            Invariant
-             (fun _ => True)
-            OnCrash
-             (fun _ => True)
-            Begin
-              let^ (fms, block) <- BFILE.read lxp ixp inum (off_remain + i*block_size) fms;
-              lrx ^(data++(read_from_block (valu_to_list block) 0 block_size))
-            Rof ^(data_init);*)
-            
-            (*for loop for reading those full blocks *)
-            let^ (data) <- (ForN_ (fun i =>
-              (pair_args_helper (fun data (_:unit) => (fun lrx => 
-              
-              let^ (fms, block) <- BFILE.read lxp ixp inum (off_remain + i*block_size) fms; (* get i'th block *)
-              lrx ^(data++(read_from_block (valu_to_list block) 0 block_size))%list (* append its contents *)
-              
-              )))) 0 num_of_full_blocks
-            (fun _:nat => (fun _ => (fun _ => (fun _ => (fun _ => True)%pred)))) (* trivial invariant *)
-            (fun _:nat => (fun _ => (fun _ => True)%pred))) ^(nil);             (* trivial crashpred *)
-            
-            let off_final := (off_remain + num_of_full_blocks * block_size) in (* offset of final block *)
-            let len_final := (len_remain - num_of_full_blocks * block_size) in (* final remaining length *)
-            let^ (fms, last_block) <- BFILE.read lxp ixp inum off_remain fms;   (* get final block *)
-            let data_final := (read_from_block (valu_to_list last_block) 0 len_final) in (* get final block data *)
-            rx ^(fms, data_init++data++data_final)%list                  (* append everything and return *)
-            }
-       }
-  } else {                                                    (* if offset is not valid, return nil *)
+      }
+    } 
+    else                                              (* If you cannot read the whole length *)
+    {    
+      let len:= (flen - off) in                               (* set length to remaining length of file *)
+      let^ (fms, block0) <- BFILE.read lxp ixp inum 0 fms;    (* get block 0 *)
+      let block_size := (get_block_size block0) in (* get block size *)
+      let block_off := (off / block_size) in              (* calculate block offset *)
+      let byte_off := (modulo off block_size) in          (* calculate byte offset *)
+      let^ (fms, first_block) <- BFILE.read lxp ixp inum off fms;   (* get first block *)
+      If(le_dec (byte_off + len) block_size)             (* if whole data is in this block *)
+      {
+        let data := (get_sublist                          (* read the data and return as list byte *)
+        (valu_to_list first_block) byte_off len) in
+        rx ^(fms, data)
+      } 
+      else                                              (* If data is in more than one block *)
+      {   
+        let data_init := (get_sublist                     (* read as much as you can from this block *)
+        (valu_to_list first_block) byte_off  
+         (block_size - byte_off)) in
+        let block_off := (block_off +1) in  (* offset of remaining part *)
+        let len_remain := (len - (block_size - byte_off)) in  (* length of remaining part *)
+        let num_of_full_blocks := (len_remain / block_size) in (* number of full blocks in length *)
+        
+        
+        (*for loop for reading those full blocks *)
+        let^ (data) <- (ForN_ (fun i =>
+          (pair_args_helper (fun data (_:unit) => (fun lrx => 
+          
+          let^ (fms, block) <- BFILE.read lxp ixp inum (block_off + i) fms; (* get i'th block *)
+          lrx ^(data++(get_sublist (valu_to_list block) 0 block_size))%list (* append its contents *)
+          
+          )))) 0 num_of_full_blocks
+        (fun _:nat => (fun _ => (fun _ => (fun _ => (fun _ => True)%pred)))) (* trivial invariant *)
+        (fun _:nat => (fun _ => (fun _ => True)%pred))) ^(nil);             (* trivial crashpred *)
+
+        rx ^(fms, data_init++data)%list                  (* append everything and return *)
+      }
+     }
+  } 
+  else                                                 (* if offset is not valid, return nil *)
+  {    
     rx ^(fms, nil)
   }
-} else {                                                      (* if read length is not valid, return nil *)
+} 
+else                                                   (* if read length is not valid, return nil *)
+{    
   rx ^(fms, nil)
 }.
 
-
-Notation "begin_addr  block_count |-->  x y" := 
-(begin_addr |-> x * (forall i, (block_count <= i) \/ (begin_addr + i |-> _ )) * (begin_addr+block_count-1) |-> v_e)%pred (at level 100).
-
+SearchAbout BFILE.memstate.
+SearchAbout GroupLog.GLog.memstate.
+SearchAbout MemLog.MLog.memstate.
+SearchAbout MemLog.MLog.mstate.
+SearchAbout mem.
+Locate "[[[".
+Print list2nmem.
 
 Theorem read_bytes_ok : forall lxp bxp ixp inum off len ms,
-    {< F Fm Fi Fd m0 m flist ilist frees f vs,
+    {< F Fm Fi Fd m0 m flist ilist frees f vs ve,
     PRE:hm
+        let block_size := (get_block_size (fst vs)) in
+        let block_off := off / block_size in
+        let byte_off := modulo off block_size in
+        let first_read_length := (block_size - byte_off) in
+        let num_of_full_reads := (len - first_read_length) / block_size in
+        let last_read_length := len - first_read_length - num_of_full_reads * block_size in
+        let file_length := length (BFILE.BFData f) in
            LOG.rep lxp F (LOG.ActiveTxn m0 m) (BFILE.MSLL ms) hm *
            [[[ m ::: (Fm * BFILE.rep bxp ixp flist ilist frees) ]]] *
            [[[ flist ::: (Fi * inum |-> f) ]]] *
-           [[[ (BFILE.BFData f) ::: (Fd * (off - (modulo off (block_size))) |-> vs )]]]*
-           [[ off < length (BFILE.BFData f) ]]
+           [[[ (BFILE.BFData f) ::: (Fd * block_off |-> vs * ((block_off + num_of_full_reads)|-> ve \/ [[file_length < off + len]]) )]]]*
+           [[ off < file_length ]]*
+           [[ 0 < len ]]
     POST:hm' RET:^(ms', r)
+          let block_size := (get_block_size (fst vs)) in
+          let block_off := off / block_size in
+          let byte_off := modulo off block_size in
+          let first_read_length := (block_size - byte_off) in
+          let num_of_full_reads := (len - first_read_length) / block_size in
+          let last_read_length := len - first_read_length - num_of_full_reads * block_size in
+          let file_length := length (BFILE.BFData f) in
            LOG.rep lxp F (LOG.ActiveTxn m0 m) (BFILE.MSLL ms') hm' *
-           [[ ((off + len <= (length (BFILE.BFData f)) /\ length r = len) 
-           \/ ( length (BFILE.BFData f) < off + len /\ length r = (length (BFILE.BFData f) - off)))
-           /\ BFILE.MSAlloc ms = BFILE.MSAlloc ms' ]]
+           [[  
+           (*[1]You read correctly*)
+           ((off + len <= file_length /\        (*[1.1]You read the full length OR*)
+               
+               (*[1.1.1]You read the first block correctly AND*)
+               (get_sublist r 0 first_read_length = get_sublist (valu_to_list (fst vs)) byte_off first_read_length ) /\ 
+               
+               (*[1.1.2]You read all middle blocks correctly AND*)
+               (forall (i:nat) bl, (num_of_full_reads < i) \/ (*[1.1.2.1]i is out of range OR*)
+                  (*[1.1.2.2]i+1'th block you read matches its contents*)
+                  ((exists F', (F' * (block_off +1 + i)|-> bl) (list2nmem m)) /\ (*[1.1.2.2.1]Block bl is in the address (block_off +1 + i) AND*)
+                  (get_sublist r (first_read_length + i*block_size) block_size (*[1.1.2.2.2]Block bl is in the address (block_off +1 + i)*)
+                      = valu_to_list (fst bl)))) /\
+               
+               (*[1.1.3]You read the last block correctly*)
+               (get_sublist r (len - last_read_length) last_read_length 
+                  = get_sublist (valu_to_list (fst ve)) 0 last_read_length))
+             \/
+             
+             (file_length < off + len /\ (*[1.2]You read as much as possible*)
+             
+                (*[1.2.1]You read the first block correctly AND*)
+                (get_sublist r 0 first_read_length = get_sublist (valu_to_list (fst vs)) byte_off first_read_length ) /\
+                
+                (*[1.2.2]You read remaining blocks correctly*)
+                (forall (i:nat) bl, ((file_length - off - first_read_length)/block_size < i) \/ (*[1.2.2.1]i is out of range OR*)
+                  (*[1.2.2.2]i+1'th block you read matches its contents*)
+                  ((exists F', (F' * (block_off +1 + i)|-> bl) (list2nmem m)) /\ (*[1.2.2.2.1]Block bl is in the address (block_off +1 + i) AND*)
+                  (get_sublist r (first_read_length + i*block_size) block_size  (*[1.2.2.2.2]Block bl is in the address (block_off +1 + i)*)
+                      = valu_to_list (fst bl))))))
+              (*[2]Memory contents didn't change*)
+              /\ BFILE.MSAlloc ms = BFILE.MSAlloc ms' ]]
     CRASH:hm'  exists ms',
            LOG.rep lxp F (LOG.ActiveTxn m0 m) (BFILE.MSLL ms') hm'
     >} read_bytes lxp ixp inum off len ms.
-
-(**
-(* It says syntax error for some reason. I couldn't find why *)
-Fixpoint read_bytes {T} lxp ixp inum (off len:nat) fms rx : prog T :=
-If (lt_dec 0 len) {                                           (* if read length > 0 *)
-  let^ (fms, flen) <- BFILE.getlen lxp ixp inum fms;          (* get file length *)
-  If (lt_dec off flen) {                                      (* if offset is inside file *)
-    If(le_dec (off+len) flen) {                               (* if you can read the whole length *)
-      let^ (fms, block) <- BFILE.read lxp ixp inum off fms;   (* get first block *)
-      let block_size := (get_block_size block) in             (* get block size *)
-      let relative_off := (modulo off block_size) in          (* calculate block offset *)
-      If(le_dec (relative_off + len) block_size) {            (* if whole data is in this block *)
-        let data := (read_from_block                          (* read the data and return as list byte *)
-        (valu_to_list (fst block)) relative_off len) in
-        rx ^(fms, data)
-      } else {                                                (* If data is in more than one block *)
-        let data:= (read_from_block                           (* read as much as you can from this block *)
-        (valu_to_list (fst block)) relative_off  
-         (block_size - relative_off)) in
-        let^ (fms, data_remaining) <- read_bytes lxp ixp inum (* read remainder from next blocks *)
-          (off + (block_size - relative_off)) 
-          (len - (block_size - relative_off)) fms;
-        rx ^(fms, (data++data_remaining))                     (* concatenate the lists and return *)
-      }
-    } else {                                                  (* If you cannot read the whole length *)
-        let^ (fms, data) <- read_bytes lxp ixp inum           (* read as much as you can and return it *)
-            off (flen - off) fms;
-        rx ^(fms, data)
-    }
-  } else {                                                    (* if offset is not valid, return nil *)
-    rx ^(fms, nil)
-  }
-} else {                                                      (* if read length is not valid, return nil *)
-  rx ^(fms, nil)
-}.
-**)
 
 End ABYTEFILE.
